src/arch/x64/X64.Semantics_s.fst
@@ -64,7 +64,6 @@ let update_reg' (r:reg) (v:nat64) (s:state) : state = {s with state = S.update_r
 
 let update_xmm' (x:xmm) (v:quad32) (s:state) : state = {s with state = S.update_xmm' x v s.state}
 
-// TODO: Mem operations
 let update_mem (ptr:int) (v:nat64) (s:state) : GTot state =
   let s' = { state = if valid_mem64 ptr s.mem then S.update_mem ptr v s.state 
   else s.state; mem = store_mem64 ptr v s.mem } in
