src/arch/x64/X64.Vale.Decls_i.fsti
@@ -315,7 +315,8 @@ let validDstAddrs128 (m:M.mem) (addr:int) (b:M.buffer128) (len:int) (memTaint:M.
     M.buffer_addr b m == addr /\
     M.valid_taint_buf128 b m memTaint t
 
-let valid_stack_slots (m:M.mem) (rsp:int) (b:M.buffer64) (num_slots:int) =
+let valid_stack_slots (m:M.mem) (rsp:int) (b:M.buffer64) (num_slots:int) (memTaint:M.memtaint) =
+    M.valid_taint_buf64 b m memTaint Public /\
     buffer_readable m b /\
     num_slots <= buffer_length b /\
     (let open FStar.Mul in
