src/arch/x64/interop/Vale_gcm_load_xor_store_buffer_win.fst
@@ -23,7 +23,7 @@ let va_pre (va_b0:va_code) (va_s0:va_state) (stack_b:buffer64)
     (valid_taint_buf128 cipher_b (va_get_mem va_s0) (va_get_memTaint va_s0) Secret) /\
     (locs_disjoint [(loc_buffer stack_b); (loc_buffer plain_b); (loc_buffer mask_b); (loc_buffer
     cipher_b)]) /\ (buffer_readable (va_get_mem va_s0) stack_b) /\ (buffer_length stack_b) >= 5 /\
-    (valid_stack_slots (va_get_mem va_s0) (va_get_reg Rsp va_s0) stack_b 0) /\ (va_get_reg Rcx
+    (valid_stack_slots (va_get_mem va_s0) (va_get_reg Rsp va_s0) stack_b 0 (va_get_memTaint va_s0)) /\ (va_get_reg Rcx
     va_s0) == (buffer_addr plain_b (va_get_mem va_s0)) /\ (va_get_reg Rdx va_s0) == (buffer_addr
     mask_b (va_get_mem va_s0)) /\ (va_get_reg R8 va_s0) == (buffer_addr cipher_b (va_get_mem
     va_s0)) /\ (va_get_reg R9 va_s0) == offset /\ (buffer_length plain_b) >= num_blocks /\
