src/arch/x64/interop/Vale_mk_quad32_lo0_be_1_buffer_win.fst
@@ -17,7 +17,7 @@ let va_pre (va_b0:va_code) (va_s0:va_state) (stack_b:buffer64)
     (va_get_ok va_s0) /\ (locs_disjoint [(loc_buffer stack_b); (loc_buffer b)]) /\ (buffer_readable
     (va_get_mem va_s0) stack_b) /\ (buffer_readable (va_get_mem va_s0) b) /\ (buffer_length b) == 1
     /\ (buffer_length stack_b) >= 2 /\ (valid_stack_slots (va_get_mem va_s0) (va_get_reg Rsp va_s0)
-    stack_b 0) /\ (va_get_reg Rcx va_s0) == (buffer_addr b (va_get_mem va_s0)) /\
+    stack_b 0 (va_get_memTaint va_s0)) /\ (va_get_reg Rcx va_s0) == (buffer_addr b (va_get_mem va_s0)) /\
     (valid_taint_buf128 b (va_get_mem va_s0) (va_get_memTaint va_s0) Secret))
 
 let va_post (va_b0:va_code) (va_s0:va_state) (va_sM:va_state) (va_fM:va_fuel) (stack_b:buffer64)
