src/arch/x64/interop/Inc32_win.fst
@@ -42,6 +42,7 @@ B.length stack_b == 16 /\ live h0 stack_b /\ buf_disjoint_from stack_b [iv_b] /\
   length_t_eq (TBase TUInt64) stack_b;
   length_t_eq (TBase TUInt128) iv_b;
   va_pre (va_code_inc32_buffer_win ()) s0 stack_b iv_b ))) =
+  assert (B.disjoint stack_b iv_b);
   length_t_eq (TBase TUInt64) stack_b;
   length_t_eq (TBase TUInt128) iv_b;
   ()
